theories/tree_borrows/step_laws/steps_retag.v
@@ -80,17 +80,17 @@ Proof.
   intros Htk. iIntros "#Hscrel Hsim".
   iApply sim_lift_base_step_both. iIntros (P_t P_s σ_t σ_s ??) "((HP_t & HP_s & Hbor) & %Hthread & %Hsafe)".
   (* exploit source to gain knowledge about stacks & that c is a valid id *)
-  specialize (pool_safe_implies Hsafe Hthread) as (c' & ot' & l' & trs1 & trs2 & [= <- <-] & [= <-] & Hcin & Hotin & Hntnin & Happly1_s & Happly2_s).
+  specialize (pool_safe_implies Hsafe Hthread) as (c' & ot' & l' & trs1 & trs2 & [= <- <-] & [= <-] & Hcin & Hotin & Hntnin & Happly1_s & Happly2_s & Hhack).
   iPoseProof "Hscrel" as "(-> & _ & Hotpub)". iClear "Hscrel".
   iPoseProof (bor_interp_get_pure with "Hbor") as "%Hp".
   destruct Hp as (Hstrs_eq & Hsnp_eq & Hsnc_eq & Hscs_eq & Hwf_s & Hwf_t & Hdom_eq).
-  odestruct (trees_equal_create_child _ _ _ _ _ _ _ _ _ _ _ _ _ _ _ _ _ _ Hstrs_eq Happly1_s) as (trs1_t&Happly1_t&Hstrs1_eq).
+  odestruct (trees_equal_create_child _ _ _ _ _ _ _ _ _ _ _ _ _ _ _ _ _ _ Hhack Hstrs_eq Happly1_s) as (trs1_t&Happly1_t&Hstrs1_eq).
   1,3: eapply Hwf_s. 2: rewrite Hsnc_eq Hsnp_eq. 1,2: eapply Hwf_t. 1: by eapply Hwf_s.
   1-2: done.
   eapply retag_step_wf_inner in Hwf_s as X. 1: destruct X as (Hwf_mid_s&Hntinmid_s).
-  2-5: done.
+  2-6: done.
   eapply retag_step_wf_inner in Hwf_t as X. 1: destruct X as (Hwf_mid_t&_).
-  5: by rewrite Hscs_eq Hsnp_eq in Happly1_t. 4: by rewrite -Hscs_eq. 2-3: setoid_rewrite <- trees_equal_same_tags; last done. 2: done. 2: by rewrite -Hsnp_eq.
+  5: by rewrite Hscs_eq Hsnp_eq in Happly1_t. 4: by rewrite -Hscs_eq. 2-3: setoid_rewrite <- trees_equal_same_tags; last done. 2: done. 2: by rewrite -Hsnp_eq. 2: done.
   edestruct trees_equal_allows_same_access as (trs2_t&Happly2_t).
   1: exact Hstrs1_eq. 1: apply Hwf_mid_s. 2: rewrite Hscs_eq. 1,2,3: apply Hwf_mid_t. 1: done. 1: by eapply mk_is_Some.
   opose proof (trees_equal_preserved_by_access _ _ Hstrs1_eq _ Happly2_s Happly2_t) as Hstrs2_eq.
@@ -151,7 +151,7 @@ Proof.
 
   iModIntro. iSplit.
   { iPureIntro. do 3 eexists. econstructor; econstructor.
-    1,3-5: repeat rewrite -?Hscs_eq -?Hsnp_eq //.
+    1,3-5: repeat rewrite -?Hscs_eq -?Hsnp_eq //. 3: done.
     all: setoid_rewrite <- trees_equal_same_tags; last done; done. }
   iIntros (e_t' efs_t σ_t') "%Hhead_t".
   destruct (head_retag_inv _ _ _ _ _ _ _ _ _ _ _ Hhead_t) as (trsX1&trsX2&->&->&Hσ_t'&Hcin_t&Hotin_t&Hntnin_t&HX1&HX2).
@@ -266,10 +266,10 @@ Proof.
          2: lia. 1: destruct l as [l1 l2]; simpl in *; subst l1; done.
        * eapply mk_is_Some, Ht3 in Hlu. rewrite Htagfresh in Hlu. by destruct Hlu.
   - (* source state wf *)
-    iPureIntro. eapply retag_step_wf_inner in Hwf_s as (Hwf_s&Hccc). 2-5: done.
+    iPureIntro. eapply retag_step_wf_inner in Hwf_s as (Hwf_s&Hccc). 2-6: done.
     eapply access_step_wf_inner in Hwf_s; done.
   - (* target state wf *)
-    iPureIntro. subst σ_t'. eapply retag_step_wf_inner in Hwf_t as (Hwf_t&Hccc). 2-5: try done.
+    iPureIntro. subst σ_t'. eapply retag_step_wf_inner in Hwf_t as (Hwf_t&Hccc). 2-6: try done.
     2: by rewrite -Hscs_eq -Hsnp_eq. simpl in Hwf_t.
     eapply access_step_wf_inner in Hwf_t. 1: done. all: simpl.
     2: by rewrite -Hscs_eq. by rewrite Hsnp_eq.
@@ -318,17 +318,17 @@ Proof.
   intros Htk. iIntros "#Hscrel Hprot Hsim".
   iApply sim_lift_base_step_both. iIntros (P_t P_s σ_t σ_s ??) "((HP_t & HP_s & Hbor) & %Hthread & %Hsafe)".
   (* exploit source to gain knowledge about stacks & that c is a valid id *)
-  specialize (pool_safe_implies Hsafe Hthread) as (c' & ot' & l' & trs1 & trs2 & [= <- <-] & [= <-] & Hcin & Hotin & Hntnin & Happly1_s & Happly2_s).
+  specialize (pool_safe_implies Hsafe Hthread) as (c' & ot' & l' & trs1 & trs2 & [= <- <-] & [= <-] & Hcin & Hotin & Hntnin & Happly1_s & Happly2_s & Hhack).
   iPoseProof "Hscrel" as "(-> & _ & Hotpub)". iClear "Hscrel".
   iPoseProof (bor_interp_get_pure with "Hbor") as "%Hp".
   destruct Hp as (Hstrs_eq & Hsnp_eq & Hsnc_eq & Hscs_eq & Hwf_s & Hwf_t & Hdom_eq).
-  odestruct (trees_equal_create_child _ _ _ _ _ _ _ _ _ _ _ _ _ _ _ _ _ _ Hstrs_eq Happly1_s) as (trs1_t&Happly1_t&Hstrs1_eq).
+  odestruct (trees_equal_create_child _ _ _ _ _ _ _ _ _ _ _ _ _ _ _ _ _ _ Hhack Hstrs_eq Happly1_s) as (trs1_t&Happly1_t&Hstrs1_eq).
   1,3: eapply Hwf_s. 2: rewrite Hsnc_eq Hsnp_eq. 1,2: eapply Hwf_t. 1: by eapply Hwf_s.
   1-2: done.
   eapply retag_step_wf_inner in Hwf_s as X. 1: destruct X as (Hwf_mid_s&Hntinmid_s).
-  2-5: done.
+  2-6: done.
   eapply retag_step_wf_inner in Hwf_t as X. 1: destruct X as (Hwf_mid_t&_).
-  5: by rewrite Hscs_eq Hsnp_eq in Happly1_t. 4: by rewrite -Hscs_eq. 2-3: setoid_rewrite <- trees_equal_same_tags; last done. 2: done. 2: by rewrite -Hsnp_eq.
+  5: by rewrite Hscs_eq Hsnp_eq in Happly1_t. 4: by rewrite -Hscs_eq. 2-3: setoid_rewrite <- trees_equal_same_tags; last done. 2: done. 2: by rewrite -Hsnp_eq. 2: done.
   edestruct trees_equal_allows_same_access as (trs2_t&Happly2_t).
   1: exact Hstrs1_eq. 1: apply Hwf_mid_s. 2: rewrite Hscs_eq. 1,2,3: apply Hwf_mid_t. 1: done. 1: by eapply mk_is_Some.
   opose proof (trees_equal_preserved_by_access _ _ Hstrs1_eq _ Happly2_s Happly2_t) as Hstrs2_eq.
@@ -396,7 +396,7 @@ Proof.
 
   iModIntro. iSplit.
   { iPureIntro. do 3 eexists. econstructor; econstructor.
-    1,3-5: repeat rewrite -?Hscs_eq -?Hsnp_eq //.
+    1,3-5: repeat rewrite -?Hscs_eq -?Hsnp_eq //. 3: done.
     all: setoid_rewrite <- trees_equal_same_tags; last done; done. }
   iIntros (e_t' efs_t σ_t') "%Hhead_t".
   destruct (head_retag_inv _ _ _ _ _ _ _ _ _ _ _ Hhead_t) as (trsX1&trsX2&->&->&Hσ_t'&Hcin_t&Hotin_t&Hntnin_t&HX1&HX2).
@@ -559,10 +559,10 @@ Proof.
          1: lia. destruct l, l_s; rewrite /shift_loc; simpl in *; f_equal; lia.
        * eapply mk_is_Some, Ht3 in Hlu. rewrite Htagfresh in Hlu. by destruct Hlu.
   - (* source state wf *)
-    iPureIntro. eapply retag_step_wf_inner in Hwf_s as (Hwf_s&Hccc). 2-5: done.
+    iPureIntro. eapply retag_step_wf_inner in Hwf_s as (Hwf_s&Hccc). 2-6: done.
     eapply access_step_wf_inner in Hwf_s; done.
   - (* target state wf *)
-    iPureIntro. subst σ_t'. eapply retag_step_wf_inner in Hwf_t as (Hwf_t&Hccc). 2-5: try done.
+    iPureIntro. subst σ_t'. eapply retag_step_wf_inner in Hwf_t as (Hwf_t&Hccc). 2-6: try done.
     2: by rewrite -Hscs_eq -Hsnp_eq. simpl in Hwf_t.
     eapply access_step_wf_inner in Hwf_t. 1: done. all: simpl.
     2: by rewrite -Hscs_eq. by rewrite Hsnp_eq.
@@ -648,17 +648,17 @@ Proof.
   iIntros "#Hscrel Hsim". 
   iApply sim_lift_base_step_both. iIntros (P_t P_s σ_t σ_s ??) "((HP_t & HP_s & Hbor) & %Hthread & %Hsafe)".
   (* exploit source to gain knowledge about stacks & that c is a valid id *)
-  specialize (pool_safe_implies Hsafe Hthread) as (c' & ot' & l' & trs1 & trs2 & [= <- <-] & [= <-] & Hcin & Hotin & Hntnin & Happly1_s & Happly2_s).
+  specialize (pool_safe_implies Hsafe Hthread) as (c' & ot' & l' & trs1 & trs2 & [= <- <-] & [= <-] & Hcin & Hotin & Hntnin & Happly1_s & Happly2_s & Hhack).
   iPoseProof "Hscrel" as "(-> & _ & Hotpub)". iClear "Hscrel".
   iPoseProof (bor_interp_get_pure with "Hbor") as "%Hp".
   destruct Hp as (Hstrs_eq & Hsnp_eq & Hsnc_eq & Hscs_eq & Hwf_s & Hwf_t & Hdom_eq).
-  odestruct (trees_equal_create_child _ _ _ _ _ _ _ _ _ _ _ _ _ _ _ _ _ _ Hstrs_eq Happly1_s) as (trs1_t&Happly1_t&Hstrs1_eq).
-  1,3: eapply Hwf_s. 2: rewrite Hsnc_eq Hsnp_eq. 1,2: eapply Hwf_t. 1: by eapply Hwf_s.
+  odestruct (trees_equal_create_child _ _ _ _ _ _ _ _ _ _ _ _ _ _ _ _ _ _ Hhack Hstrs_eq Happly1_s) as (trs1_t&Happly1_t&Hstrs1_eq).
+  1,3: eapply Hwf_s. 2: rewrite Hsnc_eq Hsnp_eq. 1,2: eapply Hwf_t. 1: by eapply Hwf_s. 
   1-2: done.
   eapply retag_step_wf_inner in Hwf_s as X. 1: destruct X as (Hwf_mid_s&Hntinmid_s).
-  2-5: done.
+  2-6: done.
   eapply retag_step_wf_inner in Hwf_t as X. 1: destruct X as (Hwf_mid_t&_).
-  5: by rewrite Hscs_eq Hsnp_eq in Happly1_t. 4: by rewrite -Hscs_eq. 2-3: setoid_rewrite <- trees_equal_same_tags; last done. 2: done. 2: by rewrite -Hsnp_eq.
+  5: by rewrite Hscs_eq Hsnp_eq in Happly1_t. 4: by rewrite -Hscs_eq. 2-3: setoid_rewrite <- trees_equal_same_tags; last done. 2: done. 2: by rewrite -Hsnp_eq. 2: done.
   edestruct trees_equal_allows_same_access as (trs2_t&Happly2_t).
   1: exact Hstrs1_eq. 1: apply Hwf_mid_s. 2: rewrite Hscs_eq. 1,2,3: apply Hwf_mid_t. 1: done. 1: by eapply mk_is_Some.
   opose proof (trees_equal_preserved_by_access _ _ Hstrs1_eq _ Happly2_s Happly2_t) as Hstrs2_eq.
@@ -716,7 +716,7 @@ Proof.
 
   iModIntro. iSplit.
   { iPureIntro. do 3 eexists. econstructor; econstructor.
-    1,3-5: repeat rewrite -?Hscs_eq -?Hsnp_eq //.
+    1,3-5: repeat rewrite -?Hscs_eq -?Hsnp_eq //. 3: done.
     all: setoid_rewrite <- trees_equal_same_tags; last done; done. }
   iIntros (e_t' efs_t σ_t') "%Hhead_t".
   destruct (head_retag_inv _ _ _ _ _ _ _ _ _ _ _ Hhead_t) as (trsX1&trsX2&->&->&Hσ_t'&Hcin_t&Hotin_t&Hntnin_t&HX1&HX2).
@@ -792,10 +792,10 @@ Proof.
        * specialize (Ht2 _ _ H1). rewrite Htagfresh in Ht2; by destruct Ht2.
        * specialize (Ht3 _ _ H1). rewrite Htagfresh in Ht3; by destruct Ht3.
   - (* source state wf *)
-    iPureIntro. eapply retag_step_wf_inner in Hwf_s as (Hwf_s&Hccc). 2-5: done.
+    iPureIntro. eapply retag_step_wf_inner in Hwf_s as (Hwf_s&Hccc). 2-6: done.
     eapply access_step_wf_inner in Hwf_s; done.
   - (* target state wf *)
-    iPureIntro. subst σ_t'. eapply retag_step_wf_inner in Hwf_t as (Hwf_t&Hccc). 2-5: try done.
+    iPureIntro. subst σ_t'. eapply retag_step_wf_inner in Hwf_t as (Hwf_t&Hccc). 2-6: try done.
     2: by rewrite -Hscs_eq -Hsnp_eq. simpl in Hwf_t.
     eapply access_step_wf_inner in Hwf_t. 1: done. all: simpl.
     2: by rewrite -Hscs_eq. by rewrite Hsnp_eq.
